\chapter{Checking Kalnay working}
\label{app:kalnay_working}

\section{Working for least squares method}
\label{sec:kalnay_working:least_squares}

Showing that the coefficients $a_1$ and $a_2$ fulfil
\begin{equation}
a_1 + a_2 = 1
\end{equation}

\subsection{Assumptions}
\label{sub:least_squares:assumptions}

\begin{itemize}
    \item $T_1$ and $T_2$ are unbiased:
    \begin{equation}
        \mathbb{E}(T_1 - T_t) = \mathbb{E}(T_2 - T_t) = 0
    \end{equation}
    \item $T_a$ is unbiased:
    \begin{equation}
        \mathbb{E}(T_a) = \mathbb{E}(T_t)
    \end{equation}
\end{itemize}

\subsection{Working}
\label{sub:least_squares:working}

We estimate $T_t$ with a linear combination of the two observations:
\begin{equation}
    T_a = a_1 T_1 + a_2 T_2,
\end{equation}
and thus
\begin{equation}
    \mathbb{E}(T_a) = \mathbb{E}(a_1 T_1 + a_2 T_2).
\end{equation}
Given that
\begin{equation}
    \mathbb{E}(X + Y) = \mathbb{E}(X) + \mathbb{E}(Y),
\end{equation}
we have
\begin{equation}
    \mathbb{E}(T_a) = \mathbb{E}(a_1 T_1) + \mathbb{E}(a_2 T_2).
\end{equation}
Given that
\begin{equation}
    \mathbb{E}(aX) = a \mathbb{E}(X),
\end{equation}
we have
\begin{equation}
    \mathbb{E}(T_a) = a_1 \mathbb{E}(T_1) + a_2 \mathbb{E}(T_2).
\end{equation}
Given that $T_1$ and $T_2$ are unbiased, we have
\begin{equation}
    \mathbb{E}(T_a) = a_1 \mathbb{E}(T_t) + a_2 \mathbb{E}(T_t).
\end{equation}
Given that $T_a$ is unbiased, we have
\begin{equation*}
    \mathbb{E}(T_t) = a_1 \mathbb{E}(T_t) + a_2 \mathbb{E}(T_t),
\end{equation*}
\begin{equation}
    \therefore a_1 + a_2 = 1
\end{equation}
